src/mqtt-packet-parser/src/ffi.fst
@@ -21,13 +21,13 @@ assume val uint8_to_c_string: u8_buffer: B.buffer U8.t -> Stack C.String.t
   (requires (fun h -> B.live h u8_buffer /\ zero_terminated_buffer_u8 h u8_buffer /\ B.length u8_buffer = 65536))
   (ensures (fun h0 ret h1 -> U32.v (C.String.strlen ret) <= 65535))
 
-assume val payload_uint8_to_c_string:
-  u8_buffer: B.buffer (B.buffer U8.t)
-  -> min_packet_size: U32.t
-  -> max_packet_size: U32.t
-  -> packet_size:
-    U32.t{U32.v packet_size >= U32.v min_packet_size && U32.v packet_size <= U32.v max_packet_size}
-  -> Stack C.String.t
-  (requires (fun h ->
-    B.live h u8_buffer /\ zero_terminated_buffer_u8 h u8_buffer ))
-  (ensures (fun h0 ret h1 -> U32.v (C.String.strlen ret) <= U32.v packet_size))
+// assume val payload_uint8_to_c_string:
+//   u8_buffer: B.buffer (B.buffer U8.t)
+//   -> min_packet_size: U32.t
+//   -> max_packet_size: U32.t
+//   -> packet_size:
+//     U32.t{U32.v packet_size >= U32.v min_packet_size && U32.v packet_size <= U32.v max_packet_size}
+//   -> Stack C.String.t
+//   (requires (fun h ->
+//     B.live h u8_buffer /\ zero_terminated_buffer_u8 h u8_buffer ))
+//   (ensures (fun h0 ret h1 -> U32.v (C.String.strlen ret) <= U32.v packet_size))
